Lynx.lean
@@ -1,6 +1,4 @@
 import Lynx.Term
-import Lynx.Contract
 import Lynx.Modules.Erlang
 import Lynx.Modules.Extensions
-import Lynx.Modules.Erlang.ListLemmas
 import Lynx.Tactic
